Fix #621
This puts in place a bug fix related to incorrect reset of RETURNDATA.
Specifically, after a `CREATE2` call in certain circumstances, the
RETURNDATA was not being reset correctly.

src/test/java/dafnyevm/GeneralStateTests.java
@@ -137,6 +137,8 @@ public class GeneralStateTests {
             "expPower256Of256_.*_0_0_0",
             "randomStatetest(52|64|320|354|367|650)_.*_0_0_0",
             "gasCostExp_.*_0_8_0",
+            // #
+            "CreateAddressWarmAfterFail_.*",
             // Unknowns
             "undefinedOpcodeFirstByte_.*_0_0_0",
             "CrashingTransaction_.*_0_0_0",
